Going to almost-working proof!

ds.v
@@ -1,5 +1,7 @@
 Require Import List.
+Require Import Arith.Plus.
 Require Import ZArith.
+Require Import FunctionalExtensionality.
 
 Definition var := nat.
 
@@ -13,8 +15,11 @@ with Ctriv : Set :=
 | Ctriv_vvar : var -> Ctriv
 | Ctriv_lam : var -> Croot -> Ctriv.
 
+Coercion Croot_exp : Cexp >-> Croot.
+Coercion Ctriv_var : var >-> Ctriv.
+
 Inductive CrootValid : Croot -> Prop :=
-| CrootValid_exp : forall e:Cexp, CexpValid e nil -> CrootValid (Croot_exp e)
+| CrootValid_exp : forall e:Cexp, CexpValid e nil -> CrootValid e
 with CexpValid : Cexp -> list var -> Prop :=
 | CexpValid_cont : forall (ksi:list var) (t:Ctriv), CtrivValid t ksi nil -> CexpValid (Cexp_cont t) ksi
 | CexpValid_app  : forall (ksi0 ksi1 ksi2:list var) (v:var) (t0 t1:Ctriv) (e:Cexp),
@@ -46,6 +51,10 @@ with Dtriv : Set :=
 | Dtriv_var : var -> Dtriv
 | Dtriv_lam : var -> Droot -> Dtriv.
 
+Coercion Droot_exp : Dexp >-> Droot.
+Coercion Dexp_triv : Dtriv >-> Dexp.
+Coercion Dtriv_var : var >-> Dtriv.
+
 Scheme Droot_mut := Induction for Droot Sort Type
 with Dexp_mut := Induction for Dexp Sort Type
 with Dtriv_mut := Induction for Dtriv Sort Type.
@@ -54,7 +63,7 @@ Hint Constructors Droot Dexp Dtriv.
 
 Fixpoint cps_transform (r:Droot) : Croot :=
 match r with
-| Droot_exp e => Croot_exp (cps_exp_transform e (fun t => Cexp_cont t))
+| Droot_exp e => cps_exp_transform e (fun t => Cexp_cont t)
 end
 with cps_exp_transform (e:Dexp) (k:Ctriv -> Cexp) : Cexp :=
 match e with
@@ -65,7 +74,7 @@ match e with
 end
 with cps_triv_transform (t:Dtriv) : Ctriv :=
 match t with
-| Dtriv_var x   => Ctriv_var x
+| Dtriv_var x   => x
 | Dtriv_lam x r => Ctriv_lam x (cps_transform r)
 end.
 
@@ -84,3 +93,174 @@ apply (Droot_mut (fun r => CrootValid (cps_transform r))
                  (fun t => forall (s:list var), CtrivValid (cps_triv_transform t) s s));
 intros; unfold good_continuation in *; eauto; simpl; intuition; eauto.
 Qed.
+
+Inductive DHroot : Set :=
+| DHroot_exp : DHexp -> DHroot
+with DHexp : Set :=
+| DHexp_app  : DHexp -> DHexp -> DHexp
+| DHexp_triv : DHtriv -> DHexp
+with DHtriv : Set :=
+| DHtriv_var  : var -> DHtriv
+| DHtriv_lam  : var -> DHroot -> DHtriv
+| DHtriv_vvar : var -> DHtriv.
+
+Scheme DHroot_mut := Induction for DHroot Sort Type
+with DHexp_mut := Induction for DHexp Sort Type
+with DHtriv_mut := Induction for DHtriv Sort Type.
+
+Coercion DHroot_exp : DHexp >-> DHroot.
+Coercion DHexp_triv : DHtriv >-> DHexp.
+Coercion DHtriv_var : var >-> DHtriv.
+
+Hint Constructors DHroot DHexp DHtriv.
+
+Fixpoint cps_htransform (r:DHroot) : Croot :=
+match r with
+| DHroot_exp e => cps_exp_htransform e (fun t => Cexp_cont t)
+end
+with cps_exp_htransform (e:DHexp) (k:Ctriv -> Cexp) : Cexp :=
+match e with
+| DHexp_app e0 e1 => cps_exp_htransform e0 (fun t0 =>
+                     cps_exp_htransform e1 (fun t1 =>
+                         Cexp_app t0 t1 0 (k (Ctriv_vvar 0))))
+| DHexp_triv t    => k (cps_triv_htransform t)
+end
+with cps_triv_htransform (t:DHtriv) : Ctriv :=
+match t with
+| DHtriv_var x   => x
+| DHtriv_vvar x  => Ctriv_vvar x
+| DHtriv_lam x r => Ctriv_lam x (cps_htransform r)
+end.
+
+Fixpoint hole_triv_number (t:DHtriv) : nat :=
+match t with
+| DHtriv_var _   => 0
+| DHtriv_lam _ _ => 0
+| DHtriv_vvar _  => 1
+end.
+
+Fixpoint hole_exp_number (e:DHexp) : nat :=
+match e with
+| DHexp_triv t    => hole_triv_number t
+| DHexp_app e0 e1 => hole_exp_number e0 + hole_exp_number e1
+end.
+
+Fixpoint hole_number (r:DHroot) : nat :=
+match r with
+| DHroot_exp e => hole_exp_number e
+end.
+
+Lemma hole_exp_valid :
+  forall e:DHexp, hole_exp_number e = 0 ->
+                  exists e':Dexp, forall k:Ctriv -> Cexp,
+                                    cps_exp_htransform e k = cps_exp_transform e' k.
+Proof.
+induction e; intros; eauto; intuition.
+inversion H; subst.
+inversion H1; subst.
+assert (hole_exp_number e1 = 0 /\ hole_exp_number e2 = 0).
+apply plus_is_O; trivial.
+destruct H0.
+simpl.
+
+specialize (IHe1 H0).
+specialize (IHe2 H3).
+destruct IHe1.
+destruct IHe2.
+exists (Dexp_app x x0).
+intros.
+simpl.
+assert ((fun t0 : Ctriv =>
+      cps_exp_htransform e2
+        (fun t1 : Ctriv => Cexp_app t0 t1 0 (k (Ctriv_vvar 0)))) = (fun t0 : Ctriv =>
+      cps_exp_transform x0
+        (fun t1 : Ctriv => Cexp_app t0 t1 0 (k (Ctriv_vvar 0))))).
+apply functional_extensionality.
+intros.
+rewrite H5.
+trivial.
+rewrite H6.
+rewrite H4.
+trivial.
+
+inversion H; subst.
+case_eq d; intros; subst; intuition.
+exists (Dexp_triv (Dtriv_var v)); auto.
+admit.
+inversion H1.
+Qed.
+
+Fixpoint nonhole_trivial (e:DHexp) : bool :=
+match e with
+| DHexp_app _ _ => false
+| DHexp_triv t  => match t with
+                   | DHtriv_var _   => true
+                   | DHtriv_lam _ _ => true
+                   | DHtriv_vvar _  => false
+                   end
+end.
+
+Fixpoint plug_triv (t:DHtriv) (e:DHexp) : DHexp :=
+match t with
+| DHtriv_var v   => DHtriv_var v
+| DHtriv_lam x r => DHtriv_lam x r
+| DHtriv_vvar _  => e
+end.
+
+Fixpoint plug_exp (e:DHexp) (e':DHexp) : DHexp :=
+match e with
+| DHexp_triv t    => plug_triv t e
+| DHexp_app e0 e1 => if nonhole_trivial e0
+                       then DHexp_app e0 (plug_exp e1 e')
+                       else DHexp_app (plug_exp e0 e') e1
+end.
+
+Fixpoint plug (r:DHroot) (e:DHexp) : DHroot :=
+match r with
+| DHroot_exp e' => plug_exp e' e
+end.
+
+Lemma cps_plugging :
+  forall (e:DHexp) (t0 t1:DHtriv),
+    not (hole_exp_number e = 0) ->
+                  cps_exp_htransform (plug_exp e (DHexp_app t0 t1)) (fun t => Cexp_cont t) =
+                  Cexp_app (cps_triv_htransform t0) (cps_triv_htransform t1) 0
+                           (cps_exp_htransform e (fun t => Cexp_cont t)).
+Proof.
+induction e; eauto; simpl; intuition.
+Admitted.
+
+Theorem super_theorem : forall r:Croot, CrootValid r -> exists dr:DHroot, cps_htransform dr = r.
+Proof.
+apply (CrootValid_mut (fun r rv => exists dr:DHroot, cps_htransform dr = r)
+                      (fun t l0 l1 tv => exists dt:DHtriv, cps_triv_htransform dt = t)
+                      (fun e l ev => exists de:DHexp, cps_exp_htransform de (fun t => Cexp_cont t) = e))
+; eauto; intuition.
+destruct H.
+exists (DHroot_exp x).
+simpl.
+admit.
+
+exists (DHtriv_vvar v).
+simpl; trivial.
+
+exists (DHtriv_var x).
+simpl; trivial.
+
+destruct H.
+exists (DHtriv_lam x x0).
+simpl.
+rewrite H; trivial.
+
+destruct H.
+exists (x).
+simpl.
+rewrite H; trivial.
+
+destruct H, H0, H1.
+exists (plug_exp x1 (DHexp_app x0 x)).
+rewrite cps_plugging.
+rewrite H.
+rewrite H0.
+rewrite H1.
+
